Add some stuff on reflection, start proving Delta_0 completeness

System_F_syn.v
@@ -176,6 +176,186 @@ Proof. exact ((FunctionalExtensionality.functional_extensionality _ _ ) (fun n =
 
 End type.
 
+Section term.
+Inductive term  : Type :=
+  | var_term : ( fin ) -> term 
+  | App : ( term   ) -> ( term   ) -> term 
+  | Abs : ( term   ) -> term .
+
+Lemma congr_App  { s0 : term   } { s1 : term   } { t0 : term   } { t1 : term   } (H1 : s0 = t0) (H2 : s1 = t1) : App  s0 s1 = App  t0 t1 .
+Proof. congruence. Qed.
+
+Lemma congr_Abs  { s0 : term   } { t0 : term   } (H1 : s0 = t0) : Abs  s0 = Abs  t0 .
+Proof. congruence. Qed.
+
+Definition upRen_term_term   (xi : ( fin ) -> fin) : ( fin ) -> fin :=
+  (up_ren) xi.
+
+Fixpoint ren_term   (xiterm : ( fin ) -> fin) (s : term ) : term  :=
+    match s return term  with
+    | var_term  s => (var_term ) (xiterm s)
+    | App  s0 s1 => App  ((ren_term xiterm) s0) ((ren_term xiterm) s1)
+    | Abs  s0 => Abs  ((ren_term (upRen_term_term xiterm)) s0)
+    end.
+
+Definition up_term_term   (sigma : ( fin ) -> term ) : ( fin ) -> term  :=
+  (scons) ((var_term ) (var_zero)) ((funcomp) (ren_term (shift)) sigma).
+
+Fixpoint subst_term   (sigmaterm : ( fin ) -> term ) (s : term ) : term  :=
+    match s return term  with
+    | var_term  s => sigmaterm s
+    | App  s0 s1 => App  ((subst_term sigmaterm) s0) ((subst_term sigmaterm) s1)
+    | Abs  s0 => Abs  ((subst_term (up_term_term sigmaterm)) s0)
+    end.
+
+Definition upId_term_term  (sigma : ( fin ) -> term ) (Eq : forall x, sigma x = (var_term ) x) : forall x, (up_term_term sigma) x = (var_term ) x :=
+  fun n => match n with
+  | S fin_n => (ap) (ren_term (shift)) (Eq fin_n)
+  | 0  => eq_refl
+  end.
+
+Fixpoint idSubst_term  (sigmaterm : ( fin ) -> term ) (Eqterm : forall x, sigmaterm x = (var_term ) x) (s : term ) : subst_term sigmaterm s = s :=
+    match s return subst_term sigmaterm s = s with
+    | var_term  s => Eqterm s
+    | App  s0 s1 => congr_App ((idSubst_term sigmaterm Eqterm) s0) ((idSubst_term sigmaterm Eqterm) s1)
+    | Abs  s0 => congr_Abs ((idSubst_term (up_term_term sigmaterm) (upId_term_term (_) Eqterm)) s0)
+    end.
+
+Definition upExtRen_term_term   (xi : ( fin ) -> fin) (zeta : ( fin ) -> fin) (Eq : forall x, xi x = zeta x) : forall x, (upRen_term_term xi) x = (upRen_term_term zeta) x :=
+  fun n => match n with
+  | S fin_n => (ap) (shift) (Eq fin_n)
+  | 0  => eq_refl
+  end.
+
+Fixpoint extRen_term   (xiterm : ( fin ) -> fin) (zetaterm : ( fin ) -> fin) (Eqterm : forall x, xiterm x = zetaterm x) (s : term ) : ren_term xiterm s = ren_term zetaterm s :=
+    match s return ren_term xiterm s = ren_term zetaterm s with
+    | var_term  s => (ap) (var_term ) (Eqterm s)
+    | App  s0 s1 => congr_App ((extRen_term xiterm zetaterm Eqterm) s0) ((extRen_term xiterm zetaterm Eqterm) s1)
+    | Abs  s0 => congr_Abs ((extRen_term (upRen_term_term xiterm) (upRen_term_term zetaterm) (upExtRen_term_term (_) (_) Eqterm)) s0)
+    end.
+
+Definition upExt_term_term   (sigma : ( fin ) -> term ) (tau : ( fin ) -> term ) (Eq : forall x, sigma x = tau x) : forall x, (up_term_term sigma) x = (up_term_term tau) x :=
+  fun n => match n with
+  | S fin_n => (ap) (ren_term (shift)) (Eq fin_n)
+  | 0  => eq_refl
+  end.
+
+Fixpoint ext_term   (sigmaterm : ( fin ) -> term ) (tauterm : ( fin ) -> term ) (Eqterm : forall x, sigmaterm x = tauterm x) (s : term ) : subst_term sigmaterm s = subst_term tauterm s :=
+    match s return subst_term sigmaterm s = subst_term tauterm s with
+    | var_term  s => Eqterm s
+    | App  s0 s1 => congr_App ((ext_term sigmaterm tauterm Eqterm) s0) ((ext_term sigmaterm tauterm Eqterm) s1)
+    | Abs  s0 => congr_Abs ((ext_term (up_term_term sigmaterm) (up_term_term tauterm) (upExt_term_term (_) (_) Eqterm)) s0)
+    end.
+
+Definition up_ren_ren_term_term    (xi : ( fin ) -> fin) (tau : ( fin ) -> fin) (theta : ( fin ) -> fin) (Eq : forall x, ((funcomp) tau xi) x = theta x) : forall x, ((funcomp) (upRen_term_term tau) (upRen_term_term xi)) x = (upRen_term_term theta) x :=
+  up_ren_ren xi tau theta Eq.
+
+Fixpoint compRenRen_term    (xiterm : ( fin ) -> fin) (zetaterm : ( fin ) -> fin) (rhoterm : ( fin ) -> fin) (Eqterm : forall x, ((funcomp) zetaterm xiterm) x = rhoterm x) (s : term ) : ren_term zetaterm (ren_term xiterm s) = ren_term rhoterm s :=
+    match s return ren_term zetaterm (ren_term xiterm s) = ren_term rhoterm s with
+    | var_term  s => (ap) (var_term ) (Eqterm s)
+    | App  s0 s1 => congr_App ((compRenRen_term xiterm zetaterm rhoterm Eqterm) s0) ((compRenRen_term xiterm zetaterm rhoterm Eqterm) s1)
+    | Abs  s0 => congr_Abs ((compRenRen_term (upRen_term_term xiterm) (upRen_term_term zetaterm) (upRen_term_term rhoterm) (up_ren_ren (_) (_) (_) Eqterm)) s0)
+    end.
+
+Definition up_ren_subst_term_term    (xi : ( fin ) -> fin) (tau : ( fin ) -> term ) (theta : ( fin ) -> term ) (Eq : forall x, ((funcomp) tau xi) x = theta x) : forall x, ((funcomp) (up_term_term tau) (upRen_term_term xi)) x = (up_term_term theta) x :=
+  fun n => match n with
+  | S fin_n => (ap) (ren_term (shift)) (Eq fin_n)
+  | 0  => eq_refl
+  end.
+
+Fixpoint compRenSubst_term    (xiterm : ( fin ) -> fin) (tauterm : ( fin ) -> term ) (thetaterm : ( fin ) -> term ) (Eqterm : forall x, ((funcomp) tauterm xiterm) x = thetaterm x) (s : term ) : subst_term tauterm (ren_term xiterm s) = subst_term thetaterm s :=
+    match s return subst_term tauterm (ren_term xiterm s) = subst_term thetaterm s with
+    | var_term  s => Eqterm s
+    | App  s0 s1 => congr_App ((compRenSubst_term xiterm tauterm thetaterm Eqterm) s0) ((compRenSubst_term xiterm tauterm thetaterm Eqterm) s1)
+    | Abs  s0 => congr_Abs ((compRenSubst_term (upRen_term_term xiterm) (up_term_term tauterm) (up_term_term thetaterm) (up_ren_subst_term_term (_) (_) (_) Eqterm)) s0)
+    end.
+
+Definition up_subst_ren_term_term    (sigma : ( fin ) -> term ) (zetaterm : ( fin ) -> fin) (theta : ( fin ) -> term ) (Eq : forall x, ((funcomp) (ren_term zetaterm) sigma) x = theta x) : forall x, ((funcomp) (ren_term (upRen_term_term zetaterm)) (up_term_term sigma)) x = (up_term_term theta) x :=
+  fun n => match n with
+  | S fin_n => (eq_trans) (compRenRen_term (shift) (upRen_term_term zetaterm) ((funcomp) (shift) zetaterm) (fun x => eq_refl) (sigma fin_n)) ((eq_trans) ((eq_sym) (compRenRen_term zetaterm (shift) ((funcomp) (shift) zetaterm) (fun x => eq_refl) (sigma fin_n))) ((ap) (ren_term (shift)) (Eq fin_n)))
+  | 0  => eq_refl
+  end.
+
+Fixpoint compSubstRen_term    (sigmaterm : ( fin ) -> term ) (zetaterm : ( fin ) -> fin) (thetaterm : ( fin ) -> term ) (Eqterm : forall x, ((funcomp) (ren_term zetaterm) sigmaterm) x = thetaterm x) (s : term ) : ren_term zetaterm (subst_term sigmaterm s) = subst_term thetaterm s :=
+    match s return ren_term zetaterm (subst_term sigmaterm s) = subst_term thetaterm s with
+    | var_term  s => Eqterm s
+    | App  s0 s1 => congr_App ((compSubstRen_term sigmaterm zetaterm thetaterm Eqterm) s0) ((compSubstRen_term sigmaterm zetaterm thetaterm Eqterm) s1)
+    | Abs  s0 => congr_Abs ((compSubstRen_term (up_term_term sigmaterm) (upRen_term_term zetaterm) (up_term_term thetaterm) (up_subst_ren_term_term (_) (_) (_) Eqterm)) s0)
+    end.
+
+Definition up_subst_subst_term_term    (sigma : ( fin ) -> term ) (tauterm : ( fin ) -> term ) (theta : ( fin ) -> term ) (Eq : forall x, ((funcomp) (subst_term tauterm) sigma) x = theta x) : forall x, ((funcomp) (subst_term (up_term_term tauterm)) (up_term_term sigma)) x = (up_term_term theta) x :=
+  fun n => match n with
+  | S fin_n => (eq_trans) (compRenSubst_term (shift) (up_term_term tauterm) ((funcomp) (up_term_term tauterm) (shift)) (fun x => eq_refl) (sigma fin_n)) ((eq_trans) ((eq_sym) (compSubstRen_term tauterm (shift) ((funcomp) (ren_term (shift)) tauterm) (fun x => eq_refl) (sigma fin_n))) ((ap) (ren_term (shift)) (Eq fin_n)))
+  | 0  => eq_refl
+  end.
+
+Fixpoint compSubstSubst_term    (sigmaterm : ( fin ) -> term ) (tauterm : ( fin ) -> term ) (thetaterm : ( fin ) -> term ) (Eqterm : forall x, ((funcomp) (subst_term tauterm) sigmaterm) x = thetaterm x) (s : term ) : subst_term tauterm (subst_term sigmaterm s) = subst_term thetaterm s :=
+    match s return subst_term tauterm (subst_term sigmaterm s) = subst_term thetaterm s with
+    | var_term  s => Eqterm s
+    | App  s0 s1 => congr_App ((compSubstSubst_term sigmaterm tauterm thetaterm Eqterm) s0) ((compSubstSubst_term sigmaterm tauterm thetaterm Eqterm) s1)
+    | Abs  s0 => congr_Abs ((compSubstSubst_term (up_term_term sigmaterm) (up_term_term tauterm) (up_term_term thetaterm) (up_subst_subst_term_term (_) (_) (_) Eqterm)) s0)
+    end.
+
+Definition rinstInst_up_term_term   (xi : ( fin ) -> fin) (sigma : ( fin ) -> term ) (Eq : forall x, ((funcomp) (var_term ) xi) x = sigma x) : forall x, ((funcomp) (var_term ) (upRen_term_term xi)) x = (up_term_term sigma) x :=
+  fun n => match n with
+  | S fin_n => (ap) (ren_term (shift)) (Eq fin_n)
+  | 0  => eq_refl
+  end.
+
+Fixpoint rinst_inst_term   (xiterm : ( fin ) -> fin) (sigmaterm : ( fin ) -> term ) (Eqterm : forall x, ((funcomp) (var_term ) xiterm) x = sigmaterm x) (s : term ) : ren_term xiterm s = subst_term sigmaterm s :=
+    match s return ren_term xiterm s = subst_term sigmaterm s with
+    | var_term  s => Eqterm s
+    | App  s0 s1 => congr_App ((rinst_inst_term xiterm sigmaterm Eqterm) s0) ((rinst_inst_term xiterm sigmaterm Eqterm) s1)
+    | Abs  s0 => congr_Abs ((rinst_inst_term (upRen_term_term xiterm) (up_term_term sigmaterm) (rinstInst_up_term_term (_) (_) Eqterm)) s0)
+    end.
+
+Lemma rinstInst_term   (xiterm : ( fin ) -> fin) : ren_term xiterm = subst_term ((funcomp) (var_term ) xiterm) .
+Proof. exact ((FunctionalExtensionality.functional_extensionality _ _ ) (fun x => rinst_inst_term xiterm (_) (fun n => eq_refl) x)). Qed.
+
+Lemma instId_term  : subst_term (var_term ) = id .
+Proof. exact ((FunctionalExtensionality.functional_extensionality _ _ ) (fun x => idSubst_term (var_term ) (fun n => eq_refl) ((id) x))). Qed.
+
+Lemma rinstId_term  : @ren_term   (id) = id .
+Proof. exact ((eq_trans) (rinstInst_term ((id) (_))) instId_term). Qed.
+
+Lemma varL_term   (sigmaterm : ( fin ) -> term ) : (funcomp) (subst_term sigmaterm) (var_term ) = sigmaterm .
+Proof. exact ((FunctionalExtensionality.functional_extensionality _ _ ) (fun x => eq_refl)). Qed.
+
+Lemma varLRen_term   (xiterm : ( fin ) -> fin) : (funcomp) (ren_term xiterm) (var_term ) = (funcomp) (var_term ) xiterm .
+Proof. exact ((FunctionalExtensionality.functional_extensionality _ _ ) (fun x => eq_refl)). Qed.
+
+Lemma compComp_term    (sigmaterm : ( fin ) -> term ) (tauterm : ( fin ) -> term ) (s : term ) : subst_term tauterm (subst_term sigmaterm s) = subst_term ((funcomp) (subst_term tauterm) sigmaterm) s .
+Proof. exact (compSubstSubst_term sigmaterm tauterm (_) (fun n => eq_refl) s). Qed.
+
+Lemma compComp'_term    (sigmaterm : ( fin ) -> term ) (tauterm : ( fin ) -> term ) : (funcomp) (subst_term tauterm) (subst_term sigmaterm) = subst_term ((funcomp) (subst_term tauterm) sigmaterm) .
+Proof. exact ((FunctionalExtensionality.functional_extensionality _ _ ) (fun n => compComp_term sigmaterm tauterm n)). Qed.
+
+Lemma compRen_term    (sigmaterm : ( fin ) -> term ) (zetaterm : ( fin ) -> fin) (s : term ) : ren_term zetaterm (subst_term sigmaterm s) = subst_term ((funcomp) (ren_term zetaterm) sigmaterm) s .
+Proof. exact (compSubstRen_term sigmaterm zetaterm (_) (fun n => eq_refl) s). Qed.
+
+Lemma compRen'_term    (sigmaterm : ( fin ) -> term ) (zetaterm : ( fin ) -> fin) : (funcomp) (ren_term zetaterm) (subst_term sigmaterm) = subst_term ((funcomp) (ren_term zetaterm) sigmaterm) .
+Proof. exact ((FunctionalExtensionality.functional_extensionality _ _ ) (fun n => compRen_term sigmaterm zetaterm n)). Qed.
+
+Lemma renComp_term    (xiterm : ( fin ) -> fin) (tauterm : ( fin ) -> term ) (s : term ) : subst_term tauterm (ren_term xiterm s) = subst_term ((funcomp) tauterm xiterm) s .
+Proof. exact (compRenSubst_term xiterm tauterm (_) (fun n => eq_refl) s). Qed.
+
+Lemma renComp'_term    (xiterm : ( fin ) -> fin) (tauterm : ( fin ) -> term ) : (funcomp) (subst_term tauterm) (ren_term xiterm) = subst_term ((funcomp) tauterm xiterm) .
+Proof. exact ((FunctionalExtensionality.functional_extensionality _ _ ) (fun n => renComp_term xiterm tauterm n)). Qed.
+
+Lemma renRen_term    (xiterm : ( fin ) -> fin) (zetaterm : ( fin ) -> fin) (s : term ) : ren_term zetaterm (ren_term xiterm s) = ren_term ((funcomp) zetaterm xiterm) s .
+Proof. exact (compRenRen_term xiterm zetaterm (_) (fun n => eq_refl) s). Qed.
+
+Lemma renRen'_term    (xiterm : ( fin ) -> fin) (zetaterm : ( fin ) -> fin) : (funcomp) (ren_term zetaterm) (ren_term xiterm) = ren_term ((funcomp) zetaterm xiterm) .
+Proof. exact ((FunctionalExtensionality.functional_extensionality _ _ ) (fun n => renRen_term xiterm zetaterm n)). Qed.
+
+End term.
+
+
+
+
+
+
+
 
 
 
@@ -184,37 +364,65 @@ End type.
 
 Global Instance Subst_type   : Subst1 (( fin ) -> type ) (type ) (type ) := @subst_type   .
 
+Global Instance Subst_term   : Subst1 (( fin ) -> term ) (term ) (term ) := @subst_term   .
+
 Global Instance Ren_type   : Ren1 (( fin ) -> fin) (type ) (type ) := @ren_type   .
+
+Global Instance Ren_term   : Ren1 (( fin ) -> fin) (term ) (term ) := @ren_term   .
 
 Global Instance VarInstance_type  : Var (fin) (type ) := @var_type  .
 
-(* Notation "x '__type'" := (var_type x) (at level 5, format "x __type") : subst_scope. *)
+Notation "x '__type'" := (var_type x) (at level 5, format "x __type") : subst_scope.
 
 (* Notation "x '__type'" := (@ids (_) (_) VarInstance_type x) (at level 5, only printing, format "x __type") : subst_scope. *)
 
 Notation "'var'" := (var_type) (only printing, at level 1) : subst_scope.
 
+Global Instance VarInstance_term  : Var (fin) (term ) := @var_term  .
+
+Notation "x '__term'" := (var_term x) (at level 5, format "x __term") : subst_scope.
+
+(* Notation "x '__term'" := (@ids (_) (_) VarInstance_term x) (at level 5, only printing, format "x __term") : subst_scope. *)
+
+Notation "'var'" := (var_term) (only printing, at level 1) : subst_scope.
+
 Class Up_type X Y := up_type : ( X ) -> Y.
 
-(* Notation "↑__type" := (up_type) (only printing) : subst_scope. *)
+Notation "↑__type" := (up_type) (only printing) : subst_scope.
 
-(* Notation "↑__type" := (up_type_type) (only printing) : subst_scope. *)
+Class Up_term X Y := up_term : ( X ) -> Y.
+
+Notation "↑__term" := (up_term) (only printing) : subst_scope.
+
+Notation "↑__type" := (up_type_type) (only printing) : subst_scope.
 
 Global Instance Up_type_type   : Up_type (_) (_) := @up_type_type   .
 
+Notation "↑__term" := (up_term_term) (only printing) : subst_scope.
+
+Global Instance Up_term_term   : Up_term (_) (_) := @up_term_term   .
+
 (* Notation "s [ sigmatype ]" := (subst_type sigmatype s) (at level 7, left associativity, only printing) : subst_scope. *)
 
-(* Notation "[ sigmatype ]" := (subst_type sigmatype) (at level 1, left associativity, only printing) : fscope. *)
+Notation "[ sigmatype ]" := (subst_type sigmatype) (at level 1, left associativity, only printing) : fscope.
 
 (* Notation "s ⟨ xitype ⟩" := (ren_type xitype s) (at level 7, left associativity, only printing) : subst_scope. *)
 
 (* Notation "⟨ xitype ⟩" := (ren_type xitype) (at level 1, left associativity, only printing) : fscope. *)
 
-Ltac auto_unfold := repeat unfold subst1,  subst2,  Subst1,  Subst2,  ids,  ren1,  ren2,  Ren1,  Ren2,  Subst_type,  Ren_type,  VarInstance_type.
+(* Notation "s [ sigmaterm ]" := (subst_term sigmaterm s) (at level 7, left associativity, only printing) : subst_scope. *)
 
-Tactic Notation "auto_unfold" "in" "*" := repeat unfold subst1,  subst2,  Subst1,  Subst2,  ids,  ren1,  ren2,  Ren1,  Ren2,  Subst_type,  Ren_type,  VarInstance_type in *.
+Notation "[ sigmaterm ]" := (subst_term sigmaterm) (at level 1, left associativity, only printing) : fscope.
 
-Ltac asimpl' := repeat first [progress rewrite ?instId_type| progress rewrite ?compComp_type| progress rewrite ?compComp'_type| progress rewrite ?rinstId_type| progress rewrite ?compRen_type| progress rewrite ?compRen'_type| progress rewrite ?renComp_type| progress rewrite ?renComp'_type| progress rewrite ?renRen_type| progress rewrite ?renRen'_type| progress rewrite ?varL_type| progress rewrite ?varLRen_type| progress (unfold up_ren, upRen_type_type, up_type_type)| progress (cbn [subst_type ren_type])| fsimpl].
+(* Notation "s ⟨ xiterm ⟩" := (ren_term xiterm s) (at level 7, left associativity, only printing) : subst_scope. *)
+
+(* Notation "⟨ xiterm ⟩" := (ren_term xiterm) (at level 1, left associativity, only printing) : fscope. *)
+
+Ltac auto_unfold := repeat unfold subst1,  subst2,  Subst1,  Subst2,  ids,  ren1,  ren2,  Ren1,  Ren2,  Subst_type,  Subst_term,  Ren_type,  Ren_term,  VarInstance_type,  VarInstance_term.
+
+Tactic Notation "auto_unfold" "in" "*" := repeat unfold subst1,  subst2,  Subst1,  Subst2,  ids,  ren1,  ren2,  Ren1,  Ren2,  Subst_type,  Subst_term,  Ren_type,  Ren_term,  VarInstance_type,  VarInstance_term in *.
+
+Ltac asimpl' := repeat first [progress rewrite ?instId_type| progress rewrite ?compComp_type| progress rewrite ?compComp'_type| progress rewrite ?instId_term| progress rewrite ?compComp_term| progress rewrite ?compComp'_term| progress rewrite ?rinstId_type| progress rewrite ?compRen_type| progress rewrite ?compRen'_type| progress rewrite ?renComp_type| progress rewrite ?renComp'_type| progress rewrite ?renRen_type| progress rewrite ?renRen'_type| progress rewrite ?rinstId_term| progress rewrite ?compRen_term| progress rewrite ?compRen'_term| progress rewrite ?renComp_term| progress rewrite ?renComp'_term| progress rewrite ?renRen_term| progress rewrite ?renRen'_term| progress rewrite ?varL_type| progress rewrite ?varL_term| progress rewrite ?varLRen_type| progress rewrite ?varLRen_term| progress (unfold up_ren, upRen_type_type, upRen_term_term, up_type_type, up_term_term)| progress (cbn [subst_type subst_term ren_type ren_term])| fsimpl].
 
 Ltac asimpl := repeat try unfold_funcomp; auto_unfold in *; asimpl'; repeat try unfold_funcomp.
 
@@ -222,8 +430,8 @@ Tactic Notation "asimpl" "in" hyp(J) := revert J; asimpl; intros J.
 
 Tactic Notation "auto_case" := auto_case (asimpl; cbn; eauto).
 
-Tactic Notation "asimpl" "in" "*" := auto_unfold in *; repeat first [progress rewrite ?instId_type in *| progress rewrite ?compComp_type in *| progress rewrite ?compComp'_type in *| progress rewrite ?rinstId_type in *| progress rewrite ?compRen_type in *| progress rewrite ?compRen'_type in *| progress rewrite ?renComp_type in *| progress rewrite ?renComp'_type in *| progress rewrite ?renRen_type in *| progress rewrite ?renRen'_type in *| progress rewrite ?varL_type in *| progress rewrite ?varLRen_type in *| progress (unfold up_ren, upRen_type_type, up_type_type in *)| progress (cbn [subst_type ren_type] in *)| fsimpl in *].
+Tactic Notation "asimpl" "in" "*" := auto_unfold in *; repeat first [progress rewrite ?instId_type in *| progress rewrite ?compComp_type in *| progress rewrite ?compComp'_type in *| progress rewrite ?instId_term in *| progress rewrite ?compComp_term in *| progress rewrite ?compComp'_term in *| progress rewrite ?rinstId_type in *| progress rewrite ?compRen_type in *| progress rewrite ?compRen'_type in *| progress rewrite ?renComp_type in *| progress rewrite ?renComp'_type in *| progress rewrite ?renRen_type in *| progress rewrite ?renRen'_type in *| progress rewrite ?rinstId_term in *| progress rewrite ?compRen_term in *| progress rewrite ?compRen'_term in *| progress rewrite ?renComp_term in *| progress rewrite ?renComp'_term in *| progress rewrite ?renRen_term in *| progress rewrite ?renRen'_term in *| progress rewrite ?varL_type in *| progress rewrite ?varL_term in *| progress rewrite ?varLRen_type in *| progress rewrite ?varLRen_term in *| progress (unfold up_ren, upRen_type_type, upRen_term_term, up_type_type, up_term_term in *)| progress (cbn [subst_type subst_term ren_type ren_term] in *)| fsimpl in *].
 
-Ltac substify := auto_unfold; try repeat (erewrite rinstInst_type).
+Ltac substify := auto_unfold; try repeat (erewrite rinstInst_type); try repeat (erewrite rinstInst_term).
 
-Ltac renamify := auto_unfold; try repeat (erewrite <- rinstInst_type).
+Ltac renamify := auto_unfold; try repeat (erewrite <- rinstInst_type); try repeat (erewrite <- rinstInst_term).
