ha2_refl.v
@@ -1,0 +1,149 @@
+(* Let's build tools to reflect Coq proofs into HA2 *)
+
+Require Import ha2.
+
+Locate "≃".
+
+Require Import Arith.
+
+Search Nat.ltb.
+
+Fixpoint closed_tm (level : fin) (t : tm) : bool :=
+  match t with
+  | var_tm n => n <? level
+  | Succ t => closed_tm level t
+  | Z => true
+  | Add t1 t2
+  | Mult t1 t2 => closed_tm level t1 && closed_tm level t2
+  end.
+
+
+Fixpoint closed_prop (t_level p_level : fin) (P : prop) : bool :=
+  match P with
+  | n ∈ P => closed_tm t_level n && closed_pred t_level p_level P
+  | all P => closed_prop (shift t_level) p_level P
+  | FORALL P => closed_prop t_level (shift p_level) P
+  | P ⇒ Q => closed_prop t_level p_level P && closed_prop t_level p_level Q
+  end
+with
+    closed_pred (t_level p_level : fin) (P : pred) : bool :=
+      match P with
+      | var_pred n => n <? p_level
+      | {{ _ | P }} => closed_prop (shift t_level) p_level P
+      end.
+
+Notation "t ≄ u" := ((t ≃ u) ⇒ ⊥)(at level 20).
+Locate "∃".
+
+Import ListNotations.
+
+Check is_true.
+
+Coercion is_true : bool >-> Sortclass.
+
+
+Fixpoint n_tm (n : nat) : tm :=
+  match n with
+  | 0 => Z
+  | S n => Succ (n_tm n)
+  end.
+
+
+Lemma subst_closed : forall σ t, closed_tm 0 t -> t[σ] = t.
+Proof.
+  induction t; simpl; asimpl; auto.
+  - intro h; inversion h.
+  - intros; rewrite IHt; auto.
+  - unfold is_true.
+    rewrite Bool.andb_true_iff.
+    intros (h1 & h2).
+    rewrite IHt1, IHt2; auto.
+  - unfold is_true.
+    rewrite Bool.andb_true_iff.
+    intros (h1 & h2).
+    rewrite IHt1, IHt2; auto.
+Qed.
+
+
+Lemma tm_pattern_at_impl : forall P Q u, tm_pattern_at u (P ⇒ Q) = (tm_pattern_at u P) ⇒ (tm_pattern_at u Q).
+Proof.
+  intros; reflexivity.
+Qed.
+
+Lemma tm_pattern_at_eq : forall t1 t2 u, tm_pattern_at u (t1 ≃ t2) = (tm_pattern_at_tm u t1) ≃ (tm_pattern_at_tm u t2).
+Proof.
+  intros; reflexivity.
+Qed.
+
+Ltac patme u := (rewrite (tm_pattern_at_subst u); repeat rewrite tm_pattern_at_impl, tm_pattern_at_eq).
+
+
+Lemma trans_apply : forall Γ t1 t2 t3,
+    Γ ⊢ t1 ≃ t2 -> Γ ⊢ t2 ≃ t3 -> Γ ⊢ t1 ≃ t3.
+Proof.
+  intros.
+  destruct (eq_dec_tm t1 t3); [subst; apply eq_refl|].
+  destruct (eq_dec_tm t2 t3); [subst; now auto|].
+  destruct (eq_dec_tm t1 t2); [subst; now auto|].
+  apply imp_elim with (P := t2 ≃ t3); auto.
+  apply imp_elim with (P := t1 ≃ t2); auto.
+  patme t3; apply forallt_elim.
+  patme t2; apply forallt_elim.
+  patme t1; apply forallt_elim.
+
+Lemma eq_add : forall Γ k l,
+    Γ ⊢ Add (n_tm k) (n_tm l) ≃ n_tm (k + l).
+Proof.
+  Search (_ + _).
+  intros Γ k l; revert k Γ; induction l; intros; simpl; rewrite Nat.add_comm; simpl.
+  - replace (Add (n_tm k) Z ≃ n_tm k) with ((Add (var_tm 0) Z ≃ (var_tm 0))[(n_tm k) ..; ids]) by (asimpl; simpl; auto).
+    apply forallt_elim.
+    apply plus_Z.
+  - apply imp_elim with (P := Succ (Add (n_tm k) (n_tm l)) ≃ Succ (n_tm (l+k))).
+    + apply imp_elim with (P := Add (n_tm k) (Succ (n_tm l)) ≃ Succ (Add (n_tm k) (n_tm l))).
+      -- Check eq_trans.
+         patme (Succ (n_tm (l+k))).
+         apply forallt_elim.
+         patme 
+         
+         pose (goal := Add (n_tm k) (Succ (n_tm l)) ≃ Succ (Add (n_tm k) (n_tm l))
+                           ⇒ Succ (Add (n_tm k) (n_tm l)) ≃ Succ (n_tm (l + k))
+                           ⇒ Add (n_tm k) (Succ (n_tm l)) ≃ Succ (n_tm (l + k))).
+         replace (Add (n_tm k) (Succ (n_tm l)) ≃ Succ (Add (n_tm k) (n_tm l))
+                      ⇒ Succ (Add (n_tm k) (n_tm l)) ≃ Succ (n_tm (l + k))
+                      ⇒ Add (n_tm k) (Succ (n_tm l)) ≃ Succ (n_tm (l + k))) with goal by reflexivity.
+         
+
+Lemma eq_norm : forall Γ vval t,
+    closed_tm 0 t ->
+    Γ ⊢ t ≃ n_tm (eval_tm vval t).
+Proof.
+  intros Γ vval t; induction t; intros; simpl; auto.
+  - inversion H.
+  - apply eq_refl.
+  - inversion H.
+    assert (h := IHt H1).
+    Locate "≃".
+    replace (Succ t ≃ Succ (n_tm (eval_tm vval t)))
+      with ((Succ t ≃ Succ (var_tm 0))[(n_tm (eval_tm vval t))..; ids]) by (asimpl; rewrite subst_closed; auto).
+    apply compr_elim.
+    eapply imp_elim with (P := t ∈ {{_ | Succ t ≃ Succ (var_tm 0) }}).
+    + replace (t ∈ ({{ _ | Succ t ≃ Succ (var_tm 0)}})
+                 ⇒ n_tm (eval_tm vval t) ∈ ({{ _ | Succ t ≃ Succ (var_tm 0)}})) with
+        ((t ∈ var_pred 0 ⇒ n_tm (eval_tm vval t) ∈ var_pred 0)[ids; {{ _ | Succ t ≃ Succ (var_tm 0)}}..]) by (asimpl; auto).
+      apply forallP_elim; auto.
+    + apply compr_intro.
+      asimpl; rewrite subst_closed; auto.
+      apply eq_refl.
+  - 
+Qed.
+
+Theorem eq_complete : forall t u,
+    closed_tm 0 t ->
+    closed_tm 0 u ->
+    [] ⊧ t ≃ u ->
+    [] ⊢ t ≃ u.
+Proof.
+  unfold "⊧".
+  simpl.
+
